providers/evercrypt/EverCrypt.Hash.fsti
@@ -266,6 +266,9 @@ val init: #a:e_alg -> (
 
 val update_multi_256: Hacl.Hash.Definitions.update_multi_st SHA2_256
 
+inline_for_extraction noextract
+val update_multi_224: Hacl.Hash.Definitions.update_multi_st SHA2_224
+
 // Note: this function relies implicitly on the fact that we are running with
 // code/lib/kremlin and that we know that machine integers and secret integers
 // are the same. In the long run, we should standardize on a secret integer type
@@ -311,6 +314,9 @@ val update_multi:
     preserves_freeable s h0 h1))
 
 val update_last_256: Hacl.Hash.Definitions.update_last_st SHA2_256
+
+inline_for_extraction noextract
+val update_last_224: Hacl.Hash.Definitions.update_last_st SHA2_224
 
 // 18-03-05 note the *new* length-passing convention!
 // 18-03-03 it is best to let the caller keep track of lengths.
@@ -396,6 +402,7 @@ val copy:
       repr s_dst h1 == repr s_src h0))
 
 val hash_256: Hacl.Hash.Definitions.hash_st SHA2_256
+val hash_224: Hacl.Hash.Definitions.hash_st SHA2_224
 
 (** @type: true
 *)
